pointers.v
@@ -256,7 +256,8 @@ Proof.
   destruct 1; inversion_clear 1; constructor; eauto using addr_refine_compose.
 Qed.
 Lemma ptr_refine_weaken Γ Γ' f f' m1 m2 m1' m2' p1 p2 σ :
-  ✓ Γ → p1 ⊑{Γ,f@m1↦m2} p2 : σ → Γ ⊆ Γ' → f ⊆ f' →
+  ✓ Γ → p1 ⊑{Γ,f@m1↦m2} p2 : σ → Γ ⊆ Γ' →
+  (∀ o o2 r τ, m1 ⊢ o : τ → f !! o = Some (o2,r) → f' !! o = Some (o2,r)) →
   (∀ o τ, m1 ⊢ o : τ → m1' ⊢ o : τ) → (∀ o τ, m2 ⊢ o : τ → m2' ⊢ o : τ) →
   (∀ o1 o2 r, f !! o1 = Some (o2,r) → index_alive m1' o1 → index_alive m2' o2) →
   p1 ⊑{Γ',f'@m1'↦m2'} p2 : σ.
